Translate another spec
Include some brief general instructions on how to do so. Could be automated
with a script relatively easily, and with some effort in Ltac as well.

src/ConcurrentFS.v
@@ -162,3 +162,85 @@ Proof.
   apply Bridge.compiler_correct.
   apply seq_file_get_attr_ok.
 Qed.
+
+(* translating spec:
+
+copy type of exists from Check
+
+s/(\(.*?\): *\(.*?\))/(\2) */g to change exists to a single product
+
+copy type of exists again
+
+s/(\(.*?\) *: *\(.*?\))/\1,/g to get the names in a let binding
+
+now copy the precondition
+
+add a fun binding for the return; copy the type from the type of rx in the spec, and then bind variables to handle the pair_args_helper
+
+copy the postcondition, with return variables now in scope
+
+copy the crash condition inside a (fun hm')
+
+add %pred scopes to the pre/post/crash conditions
+
+*)
+
+Definition read_fblock_spec (fsxp : FSLayout.fs_xparams) (inum off : addr)
+           (mscs : BFile.BFILE.memstate) :=
+  fun (a: (DiskSet.diskset) * (pred) * (pred) * (DirTree.DIRTREE.dirtree) *
+           (list string) * (BFile.BFILE.bfile) *
+           (pred) * (BFile.BFILE.datatype) * (list Inode.INODE.inode) *
+           (list addr * list addr) * (pred)) (hm: hashmap) =>
+    let '(ds, Fm, Ftop, tree, pathname, f, Fd, vs, ilist, frees, F_) := a in
+    SeqSpec
+      ((F_
+                ✶ (((Log.LOG.rep (FSLayout.FSXPLog fsxp)
+                       (SuperBlock.SB.rep fsxp) (Log.LOG.NoTxn ds)
+                       (AFS.MSLL mscs) hm
+                     ✶ ⟦⟦ (Fm ✶ DirTree.DIRTREE.rep fsxp Ftop tree ilist frees)
+                            (GenSepN.list2nmem ds !!) ⟧⟧)
+                    ✶ ⟦⟦ DirTree.DIRTREE.find_subtree pathname tree =
+                         Some (DirTree.DIRTREE.TreeFile inum f) ⟧⟧)
+                   ✶ ⟦⟦ (Fd ✶ off |-> vs)
+                          (GenSepN.list2nmem (BFile.BFILE.BFData f)) ⟧⟧))
+         ✶ ⟦⟦ PredCrash.sync_invariant F_ ⟧⟧)%pred
+      (fun (ret:  BFile.BFILE.memstate * (valu * unit)) (hm': hashmap) =>
+         let '(mscs', (r, _)) := ret in
+          F_
+                              ✶ (Log.LOG.rep (FSLayout.FSXPLog fsxp)
+                                   (SuperBlock.SB.rep fsxp)
+                                   (Log.LOG.NoTxn ds) (AFS.MSLL mscs') hm'
+                                 ✶ ⟦⟦ r = fst vs /\
+                                      AFS.MSAlloc mscs' = AFS.MSAlloc mscs ⟧⟧))%pred
+      (fun hm' =>
+         (F_
+            ✶ Log.LOG.idempred (FSLayout.FSXPLog fsxp)
+            (SuperBlock.SB.rep fsxp) ds hm')
+           ✶ ⟦⟦ exists l : list (word hashlen * {sz : addr & word sz}),
+                  hashmap_subset l hm hm' ⟧⟧)%pred.
+
+Lemma seq_read_fblock_ok : forall fsxp inum off mscs,
+    seq_hoare_double
+      (fun a => read_fblock_spec fsxp inum off mscs a)
+      (AFS.read_fblock fsxp inum off mscs).
+Proof.
+  unfold seq_hoare_double; intros.
+
+  (* work around a bug triggered by cancel *)
+  apply corr2_exists; intros.
+
+  SepAuto.hoare.
+Qed.
+
+Definition read_fblock fsxp inum off mscs :=
+  Bridge.compile (AFS.read_fblock fsxp inum off mscs).
+
+Theorem concurrent_read_fblock_ok : forall fsxp inum off mscs,
+    Bridge.concur_hoare_double
+      (fun a => Bridge.concurrent_spec (read_fblock_spec fsxp inum off mscs a))
+      (read_fblock fsxp inum off mscs).
+Proof.
+  intros.
+  apply Bridge.compiler_correct.
+  apply seq_read_fblock_ok.
+Qed.
